main: map progressed

src/TMP/EqBF/Experiment.v
@@ -5,9 +5,364 @@ Import BigStep.
 
 
 
+(*
+////////////////////////////////////////////////////////////////////////////////
+//// SECTION: MAKE_VALUE_Map /////////////////////////////////////////////////////////
+////////////////////////////////////////////////////////////////////////////////
+*)
+
+
+Print make_value_map.
+
+(*
+Refactor needed: make_value_map
+  uses to Value : list instead of (Value * Value) list
+*)
+
+Print map_insert.
+
+Lemma map_insert_unfold :
+  forall k v kl vl,
+    map_insert k v kl vl
+  = match kl with
+    | [] => match vl with
+            | [] => ([k], [v])
+            | _ :: _ => ([], [])
+            end
+    | k' :: ks =>
+        match vl with
+        | [] => ([], [])
+        | v' :: vs =>
+            if Value_ltb k k'
+            then (k :: k' :: ks, v :: v' :: vs)
+            else
+             if Value_eqb k k'
+             then (k' :: ks, v' :: vs)
+             else (k' :: (map_insert k v ks vs).1, v' :: (map_insert k v ks vs).2)
+        end
+    end.
+Proof.
+  itr.
+  des - kl; des - vl :- trv.
+Qed.
+
+Fixpoint map_insert2
+  (kv vv : Value)
+  (vl : list (Value * Value))
+  : list (Value * Value)
+  :=
+match vl with
+| [] =>  [(kv, vv)]
+| (kv', vv') :: vl' =>
+    if Value_ltb kv kv'
+    then ((kv, vv) :: (kv', vv') :: vl')
+    else
+      if Value_eqb kv kv'
+      then ((kv', vv') :: vl')
+      else ((kv', vv') :: (map_insert2 kv vv vl'))
+end.
+
+Lemma map_insert2_unfold :
+  forall kv vv vl,
+    map_insert2 kv vv vl
+  = match vl with
+    | [] =>  [(kv, vv)]
+    | (kv', vv') :: vl' =>
+        if Value_ltb kv kv'
+        then ((kv, vv) :: (kv', vv') :: vl')
+        else
+          if Value_eqb kv kv'
+          then ((kv', vv') :: vl')
+          else ((kv', vv') :: (map_insert2 kv vv vl'))
+    end.
+Proof.
+  itr.
+  des - vl; trv.
+Qed.
+
+Definition combine_unfold :
+  forall A B (l : list A) (l' : list B),
+    combine l l'
+  = match l with
+    | [] => []
+    | x :: tl => match l' with
+                 | [] => []
+                 | y :: tl' => (x, y) :: combine tl tl'
+                 end
+    end.
+Proof.
+  itr.
+  des - l; des - l' :- trv.
+Qed.
+
+Print make_value_map.
+Print combine.
+
+Fixpoint make_value_map2
+  (vl : list (Value * Value))
+  : list (Value * Value)
+  :=
+match vl with
+| [] => []
+| (kv', vv') :: vl' => map_insert2 kv' vv' (make_value_map2 vl')
+end.
+
+Lemma combine_empty :
+  forall A (kvl : list A) (vvl : list A),
+      Datatypes.length kvl = Datatypes.length vvl
+  ->  combine kvl vvl = []
+  ->  kvl = [] /\ vvl = [].
+Proof.
+  itr - A kvl vvl Hlength Hcombine.
+  rwr - combine_unfold in Hcombine.
+  case_match.
+  * smp - Hlength.
+    sym - Hlength.
+    app - length_zero_iff_nil as Hempty in Hlength.
+    sbt; spl; trv.
+  * case_match.
+    - ivs - Hlength.
+    - ivc - Hcombine.
+Qed. 
+
+Lemma map_insert_equal :
+  forall kv vv kvl vvl kvl' vvl' vl vl',
+      Datatypes.length kvl = Datatypes.length vvl
+  ->  map_insert kv vv kvl vvl = (kvl', vvl')
+  ->  combine kvl vvl = vl
+  ->  combine kvl' vvl' = vl'
+  ->  map_insert2 kv vv vl = vl'.
+Proof.
+  itr - kv vv kvl vvl kvl' vvl' vl vl' Hlength Hinsert Hcombine Hcombine'.
+  ind - vl as [| v vl].
+  * pse - combine_empty as Hempty: Value kvl vvl Hlength Hcombine.
+    des - Hempty as [Hempty_kvl Hempty_vvl].
+    sbt; clr - Hcombine.
+    ivc - Hinsert.
+    bmp.
+  * admit.
+Admitted.
+  
+
+  Theorem bs_map_insert_length1 :
+    forall k v kl vl v0,
+        Datatypes.length kl < Datatypes.length vl
+    ->  length (map_insert k v kl vl).1
+      = length (map_insert k v kl (v0 :: vl)).1.
+  Proof.
+    itr - k v kl vl v0 Hnle.
+    rwr - map_insert_unfold.
+    ind - kl as [| k1 kl IHkl]; des - vl as [| v1 vl] :- smp - Hnle; sli.
+    ass - as Hnle0: smp + Hnle; lia >
+      (Datatypes.length kl < Datatypes.length (v1 :: vl)).
+    spc - IHkl: Hnle0.
+    des > (Value_ltb k k1).
+Admitted.
+
+  Theorem bs_map_insert_length_nle :
+    forall k v kl vl,
+        Datatypes.length kl <= Datatypes.length vl
+    ->  length kl <= length (map_insert k v kl vl).1.
+  Proof.
+    (* #1 Induction List: intro/induction + simpl/lia *)
+    itr - k v kl vl Hnle.
+    ind - kl as [| k' kl IHkl]: sli |> smp.
+    (* #2 Specialize Induction: assert/specialze + simpl/lia/clear *)
+    ass - as Hnle0: smp - Hnle; lia >
+      (Datatypes.length kl ≤ Datatypes.length vl).
+    spc - IHkl: Hnle0.
+    (* #3 Case Elimination: destruct + simpl/lia *)
+    des - vl as [| v' vl]: smp - Hnle; lia.
+    (* #4 Destruct Key: destruct/apply + simpl/lia *)
+    des > (Value_ltb k k'): sli.
+    des > (Value_eqb k k'): sli |> smp + Hnle.
+    app - le_n_S.
+    
+    rwr + map_insert_unfold in IHkl.
+    des - kl as [| k'' kl]; des - vl as [| v'' vl].
+    * sli.
+    * sli.
+    * smp - Hnle. sli.
+    * 
+    des > (Value_ltb k k''): sli.
+    des > (Value_eqb k k''): sli |> smp + IHkl.
+    cbn in IHkl.
+  Admitted.
+
+Lemma make_value_map_length :
+  forall kvl vvl,
+      Datatypes.length kvl = Datatypes.length vvl
+  ->  Datatypes.length (make_value_map kvl vvl).1
+    = Datatypes.length (make_value_map kvl vvl).2.
+Proof.
+  itr - kvl vvl Hlength.
+  des - kvl as [| kv kvl]; des - vvl as [| vv vvl] :- smp - Hlength; con + smp.
+  ivc - Hlength as Hlength: H0.
+  rfl - make_value_map.
+  rwr - map_insert_unfold.
+  Search Datatypes.length.
+  des > ((make_value_map kvl vvl).1); des > ((make_value_map kvl vvl).2).
+  1-3: trv.
+  des > (Value_ltb kv v); des > (Value_eqb kv v).
+  1-3: smp; trv.
+Admitted.
+  
+Lemma make_value_map_empty_keys1 :
+  forall kvl vvl mvvl,
+      Datatypes.length kvl = Datatypes.length vvl
+  ->  make_value_map kvl vvl = ([], mvvl)
+  ->  mvvl = [].
+Proof.
+  itr - kvl vvl mvvl Hlength Hmake.
+  des - kvl as [| kv kvl]; des - vvl as [| vv vvl] :- smp - Hlength; con.
+  * bvs - Hmake.
+  * ivc - Hlength as Hlength: H0.
+    rfl - make_value_map map_insert in Hmake.
+    rwr - map_insert_unfold in Hmake.
+    des > ((make_value_map kvl vvl).1); des > ((make_value_map kvl vvl).2) :-
+      ivs - Hmake.
+    des > (Value_ltb kv v); des > (Value_eqb kv v) :- ivs - Hmake.
+Qed.
+
+
+Lemma make_value_map_empty_keys2 :
+  forall kvl vvl mvvl,
+      Datatypes.length kvl = Datatypes.length vvl
+  ->  make_value_map kvl vvl = ([], mvvl)
+  ->  kvl = [].
+Proof.
+  itr - kvl vvl mvvl Hlength Hmake.  
+  pse - make_value_map_empty_keys1 as Hmvvl: kvl vvl mvvl Hlength Hmake.
+  cwr - Hmvvl in Hmake.
+  des - kvl as [| kv kvl]; des - vvl as [| vv vvl] :- smp - Hlength; con.
+  ivc - Hlength as Hlength: H0.
+  rfl - make_value_map map_insert in Hmake.
+  rwr - map_insert_unfold in Hmake.
+  des > ((make_value_map kvl vvl).1); des > ((make_value_map kvl vvl).2) :-
+    ivs - Hmake.
+  des > (Value_ltb kv v); des > (Value_eqb kv v) :- ivs - Hmake.
+Qed.
+
+Lemma make_value_map_empty_keys :
+  forall kvl vvl mvvl,
+      Datatypes.length kvl = Datatypes.length vvl
+  ->  make_value_map kvl vvl = ([], mvvl)
+  ->  kvl = [] /\ vvl = [] /\ mvvl = [].
+Proof.
+  itr - kvl vvl mvvl Hlength Hmake.
+  ind - kvl as [| kv kvl IHkvl]; des - vvl as [| vv vvl] :- smp - Hlength; con.
+  * clr - Hlength.
+    spl; [trv | spl; [trv | idtac]].
+    bvs - Hmake.
+  * ivc - Hlength as Hlength: H0.
+    smp - Hmake.
+    rem - mkvl' mvvl' as Hmkvl Hmvvl:
+      ((make_value_map kvl vvl).1)
+      ((make_value_map kvl vvl).2).
+    ufl - map_insert in Hmake.
+  des - vvl as [| vv vvl] :- smp - Hlength; con.
+    2: {  smp - Hlength; con.
+    spl.
+    1: rfl.
+    smp - Hmake.
+    des - vvl as [| vv vvl].
+    - spl.
+      1: rfl.
+      bvs - Hmake.
+    - 
+  spl; try spl.
+  * ind - kvl as [| kv kvl IHkvl].
+    - rfl.
+    - smp - Hmake.
+Admitted.
+
+
+Lemma make_value_map_empty_keys1' :
+  forall kvl vvl mvvl,
+      Datatypes.length kvl = Datatypes.length vvl
+  ->  make_value_map kvl vvl = ([], mvvl)
+  ->  mvvl = [].
+Proof.
+  itr - kvl vvl mvvl Hlength Hmake.
+  des - kvl as [| kv kvl]; des - vvl as [| vv vvl] :- smp - Hlength; con.
+  * bvs - Hmake.
+  * ivc - Hlength as Hlength: H0.
+    rfl - make_value_map map_insert in Hmake.
+    rwr - map_insert_unfold in Hmake.
+    des > ((make_value_map kvl vvl).1); des > ((make_value_map kvl vvl).2) :-
+      ivs - Hmake.
+    des > (Value_ltb kv v); des > (Value_eqb kv v) :- ivs - Hmake.
+Qed.
+
+
+Lemma make_value_map_empty_keys2' :
+  forall kvl vvl mvvl,
+      Datatypes.length kvl = Datatypes.length vvl
+  ->  make_value_map kvl vvl = ([], mvvl)
+  ->  kvl = [].
+Proof.
+  itr - kvl vvl mvvl Hlength Hmake.
+  pse - make_value_map_empty_keys1 as Hmvvl: kvl vvl mvvl Hlength Hmake.
+  cwr - Hmvvl in *.
+  des - kvl as [| kv kvl]; des - vvl as [| vv vvl] :- smp - Hlength; con.
+  ivc - Hlength as Hlength: H0.
+  rfl - make_value_map map_insert in Hmake.
+  rwr - map_insert_unfold in Hmake.
+  psc - make_value_map_length as Hlength_make: kvl vvl Hlength.
+  des > ((make_value_map kvl vvl).1).
+  {
+    smp - Hlength_make.
+    sym - Hlength_make.
+    app - length_zero_iff_nil as Hempty in Hlength_make.
+    rwr - Hempty in *.
+    ivs - Hmake.
+  }
+  des > ((make_value_map kvl vvl).2): ivs - Hlength_make.
+  des > (Value_ltb kv v); des > (Value_eqb kv v) :- ivs - Hmake.
+Qed.
+
+Lemma make_value_map_empty_keys3' :
+  forall kvl vvl mvvl,
+      Datatypes.length kvl = Datatypes.length vvl
+  ->  make_value_map kvl vvl = ([], mvvl)
+  ->  vvl = [].
+Proof.
+  itr - kvl vvl mvvl Hlength Hmake.
+  pse - make_value_map_empty_keys1 as Hmvvl: kvl vvl mvvl Hlength Hmake.
+  pse - make_value_map_empty_keys2 as Hkvl: kvl vvl mvvl Hlength Hmake.
+  cwr - Hmvvl Hkvl in *.
+  smp - Hlength.
+  sym - Hlength.
+  app - length_zero_iff_nil as Hempty in Hlength.
+  bwr - Hempty.
+Qed.
+
+Lemma make_value_map_empty_keys' :
+  forall kvl vvl mvvl,
+      Datatypes.length kvl = Datatypes.length vvl
+  ->  make_value_map kvl vvl = ([], mvvl)
+  ->  kvl = [] /\ vvl = [] /\ mvvl = [].
+Proof.
+  itr - kvl vvl mvvl Hlength Hmake.
+  pse - make_value_map_empty_keys1 as Hmvvl: kvl vvl mvvl Hlength Hmake.
+  pse - make_value_map_empty_keys2 as Hkvl: kvl vvl mvvl Hlength Hmake.
+  pse - make_value_map_empty_keys3 as Hvvl: kvl vvl mvvl Hlength Hmake.
+  cwr - Hmvvl Hkvl Hvvl.
+  spl; [trv | spl; trv].
+Qed.
 
 
 
+
+
+
+
+
+(*
+////////////////////////////////////////////////////////////////////////////////
+//// SECTION: REMOVE /////////////////////////////////////////////////////////
+////////////////////////////////////////////////////////////////////////////////
+*)
 
 Fixpoint remove_all
   (A B : Type) (f : A -> B -> bool) (keys : list A) (l : list B) : list B
