src/TMP/EqBF/Base.v
@@ -535,12 +535,14 @@ End WellFormedMap.
 
 
 
-Import SubstSemantics.
 
 
 
 (**
 * Help
+  - map_insert_unfold
+  - make_value_map_length
+  - make_value_map_cons
   - map_insert_length_ge [NotUsing]
   - map_insert_length_le
   - make_val_map_length
@@ -567,6 +569,92 @@ NOTES:  Later change lists to maps in Syntax
 
 
 Section WellFormedMapLemmas_Help.
+
+
+
+  Lemma map_insert_unfold :
+    forall k v kl vl,
+      map_insert k v kl vl
+    = match kl with
+      | [] => match vl with
+              | [] => ([k], [v])
+              | _ :: _ => ([], [])
+              end
+      | k' :: ks =>
+          match vl with
+          | [] => ([], [])
+          | v' :: vs =>
+              if Value_ltb k k'
+              then (k :: k' :: ks, v :: v' :: vs)
+              else
+               if Value_eqb k k'
+               then (k' :: ks, v' :: vs)
+               else (k' :: (map_insert k v ks vs).1, v' :: (map_insert k v ks vs).2)
+          end
+      end.
+  Proof.
+    (* #1 Destruct Trivial: intro/destruct/trivial *)
+    itr.
+    des - kl; des - vl :- trv.
+  Qed.
+
+
+
+  Lemma make_value_map_length :
+    forall kvl vvl,
+        Datatypes.length kvl = Datatypes.length vvl
+    ->  Datatypes.length (make_value_map kvl vvl).1
+      = Datatypes.length (make_value_map kvl vvl).2.
+  Proof.
+    (* #1 Destruct Lists: intro/destruct/inversion
+        + simpl/congruence + subst/clear *)
+    itr - kvl vvl Hlength.
+    des - kvl as [| kv kvl];des - vvl as [| vv vvl]
+       :- smp - Hlength; con + smp.
+    ivc - Hlength as Hlength: H0.
+    (* #2 Unfold Map_Insert: refold/rewrite *)
+    rfl - make_value_map.
+    rwr - map_insert_unfold.
+    (* #3 Destruct Elements: destruct + trivial/simpl *)
+    des > ((make_value_map kvl vvl).1); des > ((make_value_map kvl vvl).2).
+    1-3: trv.
+    des > (Value_ltb kv v); des > (Value_eqb kv v).
+    1-3: smp; trv.
+  Admitted.
+
+
+
+  Lemma make_value_map_cons :
+    forall kv kvl vv vvl mkvl mvvl,
+        Datatypes.length kvl = Datatypes.length vvl
+    ->  make_value_map (kv :: kvl) (vv :: vvl) = (mkvl, mvvl)
+    ->  mkvl <> [] /\ mvvl <> [].
+  Proof.
+    (* #1 Unfold Map_Insert: intro/simpl/rewrite *)
+    itr - kv kvl vv vvl mkvl mvvl Hlength Hmake.
+    smp - Hmake.
+    rwr - map_insert_unfold in Hmake.
+    (* #2 Pose Length: pose + clear *)
+    psc - make_value_map_length as Hlength_make: kvl vvl Hlength.
+    (* #3 Destruct Maps: destruct
+        + simpl/symmetry/apply/rewrite/inversion/subst/split/auto *)
+    des > ((make_value_map kvl vvl).1).
+    {
+      smp - Hlength_make.
+      sym - Hlength_make.
+      app - length_zero_iff_nil as Hempty in Hlength_make.
+      rwr - Hempty in *.
+      ivs - Hmake.
+      spl; ato.
+    }
+    des > ((make_value_map kvl vvl).2): ivs - Hlength_make.
+    (* #4 Destuct Key Eq: destruct + inversion/subst/split/auto *)
+    des > (Value_ltb kv v); des > (Value_eqb kv v); ivs - Hmake; spl; ato.
+  Qed.
+
+
+
+  Import SubstSemantics.
 
 
 
@@ -598,7 +686,7 @@ Section WellFormedMapLemmas_Help.
   Proof.
     (* #1 Induction List: intro/induction + simpl/lia *)
     itr.
-    ind - vl as [| (key, var) ms IHvl]: sli |> smp.
+    ind - vl as [| (key, var) vl IHvl]: sli |> smp.
     (* #2 Destruct Key: destruct/apply + simpl/lia *)
     des > (k <ᵥ key): sli.
     des > (k =ᵥ key): sli.
@@ -653,7 +741,7 @@ Section WellFormedMapLemmas_Help.
   Proof.
     (* #1 Induction List: intro/induction + simpl/lia *)
     itr.
-    ind - vl as [| (key, var) ms IHvl]: sli |> smp.
+    ind - vl as [| (key, var) vl IHvl]: sli |> smp.
     (* #2 Destruct Key: destruct/apply + simpl/lia *)
     des > (k <ᵥ key): sli.
     des > (k =ᵥ key): sli.
@@ -788,6 +876,10 @@ End WellFormedMapLemmas_Help.
 
 
 Section WellFormedMapLemmas_Main.
+
+
+
+  Import SubstSemantics.
 
 
 
